raft-proofs/PrevLogLeaderSublogProof.v
@@ -1,0 +1,26 @@
+Require Import Arith.
+Require Import NPeano.
+Require Import List.
+Require Import Coq.Numbers.Natural.Abstract.NDiv.
+Import ListNotations.
+Require Import Sorting.Permutation.
+Require Import Omega.
+
+Require Import Util.
+Require Import Net.
+Require Import Raft.
+Require Import VerdiTactics.
+Require Import CommonTheorems.
+
+Require Import PrevLogLeaderSublogInterface.
+
+Section PrevLogLeaderSublogProof.
+  Context {orig_base_params : BaseParams}.
+  Context {one_node_params : OneNodeParams orig_base_params}.
+  Context {raft_params : RaftParams orig_base_params}.
+
+  Instance pllsi : prevLog_leader_sublog_interface.
+  Proof.
+    constructor.
+  Admitted.
+End PrevLogLeaderSublogProof.
