raft/PrevLogLeaderSublogInterface.v
@@ -1,0 +1,29 @@
+Require Import List.
+
+Require Import Net.
+Require Import Raft.
+
+Section PrevLogLeaderSublogInterface.
+  Context {orig_base_params : BaseParams}.
+  Context {one_node_params : OneNodeParams orig_base_params}.
+  Context {raft_params : RaftParams orig_base_params}.
+
+  Definition prevLog_leader_sublog (net : network) :=
+    forall leader p t leaderId prevLogIndex prevLogTerm entries leaderCommit,
+      type (nwState net leader) = Leader ->
+      In p (nwPackets net) ->
+      pBody p = AppendEntries t leaderId prevLogIndex prevLogTerm entries leaderCommit ->
+      currentTerm (nwState net leader) = prevLogTerm ->
+      exists ple, eIndex ple = prevLogIndex /\
+             eTerm ple = prevLogTerm /\
+             In ple (log (nwState net leader)).
+
+  Class prevLog_leader_sublog_interface : Prop :=
+    {
+      prevLog_leader_sublog_invariant :
+        forall net,
+          raft_intermediate_reachable net ->
+          prevLog_leader_sublog net
+    }.
+
+End PrevLogLeaderSublogInterface.
